[refactor] refactoring some proofs + notations
- Refactored a few proofs around class/nonnull/mixed to avoid
  duplication
- Sealed some notations and tried to provide enough API to use
  them nicely, couples of TODO left

theories/heap.v
@@ -35,3 +35,79 @@ Class sem_heapGS (Σ: gFunctors) := SemHeapGS {
   sem_heap_inG :> sem_heapGpreS Σ;
   sem_heap_name: gname;
 }.
+
+Section definitions.
+  Context `{hG: !sem_heapGS Σ}.
+
+  Definition loc_mapsto_def (ℓ: loc) (t: tag)
+    (iFs: gmapO string (laterO (sem_typeO Σ))) :=
+    (gmap_view_frag ℓ DfracDiscarded (t, iFs)).
+
+  Definition mapsto_def (ℓ: loc) (t: tag)
+    (iFs: gmapO string (laterO (sem_typeO Σ))) :=
+    own (@sem_heap_name _ hG) (loc_mapsto_def ℓ t iFs).
+
+  Definition loc_mapsto_aux : seal (@loc_mapsto_def). Proof. by eexists. Qed.
+  Definition loc_mapsto := loc_mapsto_aux.(unseal).
+  Definition loc_mapsto_eq : @loc_mapsto = @loc_mapsto_def := loc_mapsto_aux.(seal_eq).
+
+  Definition mapsto_aux : seal (@mapsto_def). Proof. by eexists. Qed.
+  Definition mapsto := mapsto_aux.(unseal).
+  Definition mapsto_eq : @mapsto = @mapsto_def := mapsto_aux.(seal_eq).
+End definitions.
+
+Notation "l  ↪ '(' t ',' iFs ')'" := (loc_mapsto l t iFs)
+  (at level 20, format "l  ↪ '(' t ',' iFs ')'") : bi_scope.
+
+Notation "l ↦ '(' t ',' iFs ')'" := (mapsto l t iFs)
+  (at level 20, format "l ↦ '(' t ',' iFs ')'") : bi_scope.
+
+Section sem_heap.
+  Context `{hG: !sem_heapGS Σ}.
+
+	Lemma mapsto_contractive
+    (l: loc)
+    (t: tag)
+    (f: (lang_ty -d> sem_typeO Σ) → gmapO string (laterO (sem_typeO Σ )))
+    `{hf: Contractive f}:
+  Contractive (λ i, mapsto l t (f i)).
+  Proof.
+    move => n i1 i2 hdist.
+    rewrite mapsto_eq /mapsto_def /loc_mapsto_def.
+    do 3 f_equiv.
+    by apply hf.
+  Qed.
+
+  Global Instance mapsto_persistent l t iFs: Persistent (mapsto l t iFs).
+  Proof.
+    rewrite mapsto_eq /mapsto_def /loc_mapsto_def.
+    by apply _.
+  Qed.
+
+  Lemma sem_heap_own_valid_2 sh l t iFs:
+    own sem_heap_name (gmap_view_auth (DfracOwn 1) sh) -∗
+    l ↦ (t, iFs) -∗
+    sh !! l ≡ Some (t, iFs).
+  Proof.
+    rewrite mapsto_eq /mapsto_def /loc_mapsto_def.
+    iIntros "H● H◯".
+    iDestruct (own_valid_2 with "H● H◯") as "#Hv".
+    rewrite gmap_view_both_validI.
+    by iDestruct "Hv" as "[_ HΦ]".
+  Qed.
+
+  Lemma sem_heap_own_update new sh t iFs:
+    sh !! new = None →
+    (gmap_view_auth (DfracOwn 1) sh ~~>
+      gmap_view_auth (DfracOwn 1) (<[new:=(t, iFs)]> sh) ⋅ (new ↪ (t, iFs))%I) →
+    own sem_heap_name (gmap_view_auth (DfracOwn 1) sh) -∗
+    |==> own sem_heap_name ((gmap_view_auth (DfracOwn 1) (<[new:=(t, iFs)]> sh)) ⋅
+           (new  ↪ (t, iFs))%I).
+  Proof.
+    rewrite loc_mapsto_eq /loc_mapsto_def  => hnew h.
+    iIntros "H●".
+    iMod (own_update with "H●") as "H";
+      first by apply (gmap_view_alloc _ new DfracDiscarded (t, iFs)).
+    by iModIntro.
+  Qed.
+End sem_heap.
